minor simplifications

example_iquicksort.v
@@ -11,9 +11,9 @@ From infotheo Require Import ssr_ext.
 (*                                                                            *)
 (*    partl p (s, t) u == partition u into (x, y) w.r.t. pivot p and returns  *)
 (*                        (s ++ x, t ++ y)                                    *)
-(*    tr_partl p s t u == tail-recursive version of partl; this is a          *)
-(*                        computation of type M (seq E * seq E * seq E) where *)
-(*                        E is the type of the values in the array monad      *)
+(* qperm_partl p s t u == fusion of qperm and partl; this is a computation    *)
+(*                        of type M (seq E * seq E * seq E) where E is the    *)
+(*                        type of the values in the array monad               *)
 (* ipartl p i ny nz nx == partition the array stored at i w.r.t. the pivot p, *)
 (*                        the array is yz ++ zs ++ xs where the lengths of    *)
 (*                        yz, zs, xs are resp. ny, nz, nx; it returns the     *)
@@ -42,18 +42,18 @@ Local Open Scope tuple_ext_scope.
 From infotheo Require Import ssrZ.
 Require Import ZArith.
 
-(* TODO: equip Z with an ssr order *)
+(* NB: to appear in the next version of infotheo *)
+Lemma addZAC : right_commutative Zplus. Proof. by move=> ? ? ?; ring. Qed.
+
+Lemma addZCA : left_commutative Zplus. Proof. by move=> ? ? ?; ring. Qed.
+
 Lemma neq_Zlt (a b : Z) : (a != b) <-> (a < b)%Z \/ (b < a)%Z.
 Proof.
 split => [/eqP/not_Zeq//|[ab|ba]].
 - exact/eqP/ltZ_eqF.
 - exact/eqP/gtZ_eqF.
 Qed.
-
-(* TODO: move to infotheo *)
-Lemma addZAC : right_commutative Zplus. Proof. by move=> ? ? ?; ring. Qed.
-
-Lemma addZCA : left_commutative Zplus. Proof. by move=> ? ? ?; ring. Qed.
+(* /NB: to appear in the next version of infotheo *)
 
 Definition apply_pair_snd (M : monad) (A B C : UU0) (f : B -> M C) (ab : A * B)
     : M (A * C)%type :=
@@ -106,15 +106,17 @@ Local Open Scope zarith_ext_scope.
 
 Section partl.
 Variable (d : unit) (E : orderType d) (M : plusArrayMonad E Z_eqType).
+Implicit Types p : E.
 
-Fixpoint partl (p : E) (s : (seq E * seq E)%type) (xs : seq E)
+(* tail-recursive *)
+Fixpoint partl p (s : (seq E * seq E)%type) (xs : seq E)
     : (seq E * seq E)%type :=
   if xs is x :: xs then
     (if x <= p then partl p (rcons s.1 x, s.2) xs
               else partl p (s.1, rcons s.2 x) xs)
   else s.
 
-Lemma partlE s t p u : let x := partition p u in
+Let partlE s t p u : let x := partition p u in
   partl p (s, t) u = (s ++ x.1, t ++ x.2).
 Proof.
 elim: u p s t => [|h tl ih] /= p a b; first by rewrite !cats0.
@@ -126,21 +128,59 @@ Proof. by rewrite partlE /=; case: partition. Qed.
 
 End partl.
 
-Section tr_partl.
+Section dispatch.
 Variable (d : unit) (E : orderType d) (M : plusArrayMonad E Z_eqType).
 
-Fixpoint tr_partl (p : E) (ys zs xs : seq E) : M (seq E * seq E)%type :=
+Definition dispatch (x p : E) '(ys, zs, xs) : M (seq E * seq E * seq E)%type :=
+  if x <= p then
+    qperm zs >>= (fun zs' => Ret (rcons ys x, zs', xs))
+  else
+    qperm (rcons zs x) >>= (fun zs' => Ret (ys, zs', xs)).
+
+Lemma commute_dispatch_writeList i p ys zs xs x A
+    (f : seq E * seq E * seq E -> M A) :
+  commute (dispatch x p (ys, zs, xs)) (writeList i xs)
+          (fun x (_ : unit) => f x).
+Proof.
+apply: commute_plus; rewrite /dispatch; case: ifPn => xp.
+  have [syn syn_qperm] := nondetPlus_sub_qperm M zs.
+  exists (ndBind syn (fun s => ndRet (rcons ys x, s, xs))).
+  by rewrite /= syn_qperm.
+have [syn syn_qperm] := nondetPlus_sub_qperm M (rcons zs x).
+exists (ndBind syn (fun s => ndRet (ys, s, xs))).
+by rewrite /= syn_qperm.
+Qed.
+
+Lemma dispatch_writeList_cat (i : Z) (x p : E) (ys zs xs : seq E)
+  D (k : nat -> nat -> nat -> M D) :
+  dispatch x p (ys, zs, xs) >>= write3L i >>= uncurry3 k =
+  dispatch x p (ys, zs, xs) >>= (fun '(ys', zs', xs) =>
+    writeList i (ys' ++ zs') >> writeList (i + (size (ys' ++ zs'))%:Z) xs >>
+    k (size ys') (size zs') (size xs)).
+Proof.
+rewrite bindA.
+bind_ext => [[[ys' zs']] xs'].
+by rewrite -writeList_cat -catA /write3L bindA bindretf.
+Qed.
+
+End dispatch.
+Arguments dispatch {d E M}.
+
+Section qperm_partl.
+Variable (d : unit) (E : orderType d) (M : plusArrayMonad E Z_eqType).
+
+Fixpoint qperm_partl (p : E) (ys zs xs : seq E) : M (seq E * seq E)%type :=
   if xs is x :: xs then
-    (if x <= p then qperm zs >>= ((tr_partl p (rcons ys x))^~ xs)
-              else qperm (rcons zs x) >>= ((tr_partl p ys)^~ xs))
+    (if x <= p then qperm zs >>= ((qperm_partl p (rcons ys x))^~ xs)
+              else qperm (rcons zs x) >>= ((qperm_partl p ys)^~ xs))
   else Ret (ys, zs).
 
-Lemma nondetPlus_sub_tr_partl p (s : seq E) a b :
-  nondetPlus_sub (tr_partl p a b s).
+Lemma nondetPlus_sub_qperm_partl p (s : seq E) a b :
+  nondetPlus_sub (qperm_partl p a b s).
 Proof.
-elim: s p a b => [p a b|h t ih p a b].
+elim: s p a b => [p a b|h t ih p a b /=].
   by exists (ndRet (a, b)).
-rewrite /=; case: ifPn => hp.
+case: ifPn => hp.
   have [syn synE] := nondetPlus_sub_qperm M b.
   exists (ndBind syn (fun zs' => sval (ih p (rcons a h) zs'))) => /=.
   rewrite synE /=.
@@ -153,36 +193,16 @@ bind_ext => zs' /=.
 by case: ih.
 Qed.
 
-Definition dispatch (x p : E) '(ys, zs, xs) : M (seq E * seq E * seq E)%type :=
-  if x <= p then qperm zs >>= (fun zs' => Ret (rcons ys x, zs', xs))
-            else qperm (rcons zs x) >>= (fun zs' => Ret (ys, zs', xs)).
-
-Lemma tr_partl_dispatch (p x : E) (ys zs xs : seq E) :
-  tr_partl p ys zs (x :: xs) =
-  dispatch x p (ys, zs, xs) >>= uncurry3 (tr_partl p).
+Lemma qperm_partl_dispatch (p x : E) (ys zs xs : seq E) :
+  qperm_partl p ys zs (x :: xs) =
+  dispatch x p (ys, zs, xs) >>= uncurry3 (qperm_partl p).
 Proof.
-rewrite /dispatch {1}/tr_partl.
-by case: ifPn => _;
-  rewrite bindA; bind_ext => s; rewrite bindretf.
+rewrite /dispatch {1}/qperm_partl.
+by case: ifPn => _; rewrite bindA; bind_ext => s; rewrite bindretf.
 Qed.
 
-Lemma commute_dispatch_writeList i p ys zs xs x A (f : _ -> M A):
-  commute (dispatch x p (ys, zs, xs))
-          (writeList (i + (size ys)%:Z + (size zs)%:Z + 1) xs)
-          (fun x (_ : unit) => f x).
-Proof.
-apply: commute_plus; rewrite /dispatch; case: ifPn => xp.
-  have [syn syn_qperm] := nondetPlus_sub_qperm M zs.
-  exists (ndBind syn (fun s => ndRet (rcons ys x, s, xs))).
-  by rewrite /= syn_qperm.
-have [syn syn_qperm] := nondetPlus_sub_qperm M (rcons zs x).
-exists (ndBind syn (fun s => ndRet (ys, s, xs))).
-by rewrite /= syn_qperm.
-Qed.
-
-End tr_partl.
-Arguments tr_partl {d E M}.
-Arguments dispatch {d E M}.
+End qperm_partl.
+Arguments qperm_partl {d E M}.
 
 Section ipartl.
 Variable (d : unit) (E : orderType d) (M : plusArrayMonad E Z_eqType).
@@ -205,7 +225,7 @@ Fixpoint ipartl (p : E) (i : Z) (ny nz : nat) (nx : nat) : M (nat * nat)%type :=
 Lemma ipartl_guard (p : E) (i : Z) ny nz (nx : nat) :
   ipartl p i ny nz nx =
   ipartl p i ny nz nx >>= (fun '(a, b) =>
-    (guard ((a <= nx + ny + nz) && (b <= nx + ny + nz))%nat >> Ret (a, b))) :> M _.
+    (guard ((a <= nx + ny + nz) && (b <= nx + ny + nz))%nat >> Ret (a, b))).
 Proof.
 elim: nx ny nz => [ny nz|n ih ny nz].
   by rewrite /= bindretf add0n leq_addr leq_addl guardT bindskipf.
@@ -215,46 +235,6 @@ rewrite /= [in RHS]bindA; bind_ext => x; case: ifPn => xp.
   by under eq_bind do rewrite -addSnnS.
 - rewrite [in LHS]ih.
   by under [in RHS]eq_bind do rewrite addSnnS -addnA addSnnS addnA.
-Qed.
-
-Lemma write3L_ipartl (i : Z) (p : E) (ys zs xs : seq E) :
-  (forall ys zs,
-    (writeList i (ys ++ zs ++ xs) >> ipartl p i (size ys) (size zs) (size xs))
-    `<=`
-    (tr_partl p ys zs xs >>= write2L i)) ->
-  write3L i (ys, zs, xs) >>= uncurry3 (ipartl p i)
-  `<=`
-  uncurry3 (tr_partl p) (ys, zs, xs) >>= write2L i.
-Proof.
-move=> h.
-apply: refin_trans (h ys zs).
-rewrite bindA bindretf.
-exact: refin_refl.
-Qed.
-
-Lemma dispatch_write3L_ipartl (i : Z) (x p : E) (ys zs xs : seq E) :
-  (forall ys zs,
-    writeList i (ys ++ zs ++ xs) >> ipartl p i (size ys) (size zs) (size xs)
-    `<=`
-    (tr_partl p ys zs xs >>= write2L i)) ->
-  dispatch x p (ys, zs, xs) >>= write3L i >>= uncurry3 (ipartl p i)
-  `<=`
-  dispatch x p (ys, zs, xs) >>= uncurry3 (tr_partl p) >>= write2L i.
-Proof.
-move=> h; rewrite 2!bindA /dispatch; case: ifPn => _;
-  by rewrite 2!bindA /refin refin_bindl => // {}zs;
-     rewrite 2!bindretf; exact: write3L_ipartl h.
-Qed.
-
-Lemma dispatch_writeList_cat (i : Z) (x p : E) (ys zs xs : seq E) :
-  dispatch x p (ys, zs, xs) >>= write3L i >>= uncurry3 (ipartl p i) =
-  dispatch x p (ys, zs, xs) >>= (fun '(ys', zs', xs) =>
-    writeList i (ys' ++ zs') >> writeList (i + (size (ys' ++ zs'))%:Z) xs >>
-    ipartl p i (size ys') (size zs') (size xs)).
-Proof.
-rewrite bindA.
-bind_ext => [[[ys' zs']] xs'].
-by rewrite /write3L !bindA catA writeList_cat bindretf bindA.
 Qed.
 
 Definition dipartlT (y z x : nat) :=
@@ -283,6 +263,29 @@ case: Bool.bool_dec => [nanb|].
 by move/negP; rewrite negb_and => /orP[|] /negP.
 Qed.
 Local Close Scope mprog.
+
+Section refin_dispatch_write3L_ipartl.
+Variables (i : Z) (p : E) (xs : seq E).
+Hypothesis ih : forall ys zs,
+  writeList i (ys ++ zs ++ xs) >> ipartl p i (size ys) (size zs) (size xs)
+  `<=` qperm_partl p ys zs xs >>= write2L i.
+
+Let refin_write3L_ipartl ys zs :
+  write3L i (ys, zs, xs) >>= uncurry3 (ipartl p i)
+  `<=` uncurry3 (qperm_partl p) (ys, zs, xs) >>= write2L i.
+Proof.
+by apply: refin_trans (ih _ _); rewrite bindA bindretf; exact: refin_refl.
+Qed.
+
+Lemma refin_dispatch_write3L_ipartl x ys zs :
+  dispatch x p (ys, zs, xs) >>= write3L i >>= uncurry3 (ipartl p i)
+  `<=` dispatch x p (ys, zs, xs) >>= uncurry3 (qperm_partl p) >>= write2L i.
+Proof.
+by rewrite 2!bindA /dispatch; case: ifPn => _;
+  rewrite 2!bindA /refin refin_bindl => // zs';
+     rewrite 2!bindretf; exact: refin_write3L_ipartl.
+Qed.
+End refin_dispatch_write3L_ipartl.
 
 End ipartl.
 Arguments ipartl {d E M}.
@@ -429,36 +432,22 @@ Qed.
 
 End ssplits.
 
-Section slowsort.
-Variable M : plusMonad.
-Variables (d : unit) (E : orderType d).
-
-Lemma refin_partition_slowsort (p : E) (s : seq E) :
-  Ret (partition p s) >>= (fun '(a, b) =>
-  slowsort a >>= (fun a' => slowsort b >>= (fun b' => Ret (a' ++ p :: b'))))
-  `<=`
-  (slowsort (p :: s) : M _).
-Proof.
-rewrite slowsort_splits.
-apply: refin_trans; first exact/refin_bindr/(partition_spec M p s).
-rewrite bindA; apply: refin_bindl => -[a b].
-rewrite assertE (bindA _ (fun _ => Ret (a, b))) bindretf /= bindA.
-exact: refin_refl.
-Qed.
-
-End slowsort.
-
-Section ssplits_iqsort.
+(* top of page 11 *)
+Section derivation_qperm_partl_ipartl.
 Variable (d : unit) (E : orderType d) (M : plusArrayMonad E Z_eqType).
+Implicit Types i : Z.
 
 (* page 11 step 4 *)
-Lemma qperm_preserves_length (i : Z) (x p : E) (ys zs xs : seq E) :
+Lemma qperm_preserves_length i (x p : E) (ys zs xs : seq E)
+    D (k : nat -> nat -> nat -> M D) :
   dispatch x p (ys, zs, xs) >>= (fun '(ys', zs', xs) =>
-    writeList i (ys' ++ zs') >> writeList (i + (size (ys' ++ zs'))%:Z) xs >>
-    ipartl p i (size ys') (size zs') (size xs)) =
+    writeList i (ys' ++ zs') >>
+      writeList (i + (size (ys' ++ zs'))%:Z) xs >>
+        k (size ys') (size zs') (size xs)) =
   writeList (i + (size ys)%:Z + (size zs)%:Z + 1) xs >>
     dispatch x p (ys, zs, xs) >>= (fun '(ys', zs', xs) =>
-    writeList i (ys' ++ zs') >> ipartl p i (size ys') (size zs') (size xs)) :> M _.
+      writeList i (ys' ++ zs') >>
+        k (size ys') (size zs') (size xs)) :> M _.
 Proof.
 rewrite [in RHS]bindA.
 rewrite -commute_dispatch_writeList.
@@ -467,14 +456,13 @@ rewrite /dispatch.
 case: ifPn => xp.
   rewrite !bindA.
   under eq_bind do rewrite bindretf.
-  under [in RHS]eq_bind do rewrite bindretf.
   under eq_bind do rewrite -writeList_cat.
-  under [in RHS]eq_bind do rewrite -bindA.
-  under [in RHS]eq_bind do rewrite -2!addZA.
+  under [in RHS]eq_bind do rewrite bindretf.
+  under [in RHS]eq_bind do rewrite -bindA -2!addZA.
   rewrite [RHS](qperm_preserves_size2 zs (fun a b =>
     (writeList (i + ((size ys)%:Z + (b%:Z + 1))) xs >>
     writeList i ((rcons ys x) ++ a)) >>
-    ipartl p i (size (rcons ys x)) (size a) (size xs))).
+    k (size (rcons ys x)) (size a) (size xs))).
   bind_ext => zs' /=.
   rewrite (_ : (_ + (_ + 1))%Z = (size (ys ++ x :: zs'))%:Z); last first.
     by rewrite size_cat /= intRD natZS -add1Z (addZC 1%Z).
@@ -483,204 +471,169 @@ case: ifPn => xp.
   by rewrite writeList_cat -cats1 -catA.
 rewrite !bindA.
 under eq_bind do rewrite bindretf.
-under [in RHS]eq_bind do rewrite bindretf.
 under eq_bind do rewrite -writeList_cat.
-under [in RHS]eq_bind do rewrite -bindA.
-under [in RHS]eq_bind do rewrite -2!addZA.
+under [in RHS]eq_bind do rewrite bindretf.
+under [in RHS]eq_bind do rewrite -bindA -2!addZA.
 rewrite -Z_S -(size_rcons zs x).
 rewrite [RHS](qperm_preserves_size2 (rcons zs x) (fun a b =>
   (writeList (i + ((size ys)%:Z + b%:Z)) xs >>
-  writeList i (ys ++ a)) >> ipartl p i (size ys) (size a) (size xs))).
+  writeList i (ys ++ a)) >> k (size ys) (size a) (size xs))).
 bind_ext => zs' /=.
 rewrite (_ : (_ + (_ + _))%Z = (i + (size (ys ++ zs'))%:Z)%Z); last first.
   by rewrite size_cat /= intRD.
 by rewrite -writeListC ?writeList_cat//; exact: leZZ.
 Qed.
 
-(* page11 top derivation *)
-Lemma tr_partl_writeList (p x : E) (ys zs xs : seq E) (i : Z) :
+Lemma refin_qperm_partl_writeList (p x : E) (ys zs xs : seq E) i :
   (forall ys zs,
-       (writeList i (ys ++ zs ++ xs) >> ipartl p i (size ys) (size zs) (size xs) : M _)
-       `<=`
-       (tr_partl p ys zs xs >>= write2L i)) ->
-  (writeList (i + (size ys)%:Z + (size zs)%:Z + 1)%Z xs >>
-   if x <= p then qperm zs >>= (fun zs' => writeList i (ys ++ x :: zs') >>
-     ipartl p i (size ys + 1) (size zs') (size xs))
-   else qperm (rcons zs x) >>= (fun zs' => writeList i (ys ++ zs') >>
-     ipartl p i (size ys) (size zs') (size xs)) : M _)
+     writeList (M := M) i (ys ++ zs ++ xs) >>
+       ipartl p i (size ys) (size zs) (size xs)
+     `<=` qperm_partl p ys zs xs >>= write2L i) ->
+  (writeList (M := M) (i + (size ys)%:Z + (size zs)%:Z + 1)%Z xs >>
+    if x <= p then qperm zs >>= (fun zs' => writeList i (ys ++ x :: zs') >>
+      ipartl p i (size ys).+1 (size zs') (size xs))
+    else qperm (rcons zs x) >>= (fun zs' => writeList i (ys ++ zs') >>
+      ipartl p i (size ys) (size zs') (size xs)))
   `<=`
-  tr_partl p ys zs (x :: xs) >>= write2L i.
+  qperm_partl p ys zs (x :: xs) >>= write2L i.
 Proof.
-move=> h; rewrite tr_partl_dispatch.
-apply: refin_trans; last exact: (dispatch_write3L_ipartl _ _ _ h).
+move=> ih; rewrite qperm_partl_dispatch.
+apply: refin_trans; last exact: (refin_dispatch_write3L_ipartl ih).
 rewrite dispatch_writeList_cat.
 rewrite qperm_preserves_length.
 rewrite /dispatch bindA.
 apply refin_bindl => -[].
-case: ifPn => xp. (* TODO:  *)
-- rewrite bindA /refin -alt_bindDr.
-  bind_ext => s.
-  by rewrite bindretf size_rcons addn1 -cat1s catA cats1 altmm.
-- rewrite bindA /refin -alt_bindDr.
-  bind_ext => s.
-  by rewrite bindretf altmm.
+case: ifPn => xp; rewrite bindA; apply: refin_bindl => zs'.
+- by rewrite bindretf size_rcons -cats1 -catA /=; exact: refin_refl.
+- by rewrite bindretf; exact: refin_refl.
 Qed.
 
-End ssplits_iqsort.
+End derivation_qperm_partl_ipartl.
 
-Section fsplits.
-Variable (d : unit) (E : orderType d) (M : plusArrayMonad E Z_eqType).
+Section refin_qperm_partl.
+Variables (d : unit) (E : orderType d) (M : plusArrayMonad E Z_eqType).
 
-Lemma gt0_flatten A (s : seq A) (f : A -> A) : (0 < size s)%nat ->
-  (0 < size (flatten [seq [:: f y] | y <- s]))%nat.
-Proof. by case: s. Qed.
-
-Lemma perm_eq_flatten_map (A : eqType) (s : seq A) (f g : A -> A) :
-  perm_eq (flatten [seq [:: f y; g y] | y <- s])
-          (flatten [seq [:: f y] | y <- s] ++ flatten [seq [:: g y] | y <- s]).
+Let refin_qperm_partl_helper a b p xs :
+  (apply_triple_snd qperm >=> uncurry3 (qperm_partl p)) (a, b, xs) `<=`
+  apply_pair_snd (M := M) qperm (partl (p : E) (a, b) xs).
 Proof.
-elim: s f g => // h t ih f g.
-rewrite /=.
-rewrite -[in X in perm_eq _ X](cat1s (f h)).
-rewrite -[in X in perm_eq _ X](cat1s (g h)).
-rewrite catA.
-apply: (@perm_trans _ (([:: f h] ++ [:: g h]) ++
-                        flatten [seq [:: f y] | y <- t] ++
-                        flatten [seq [:: g y] | y <- t])); last first.
-  rewrite perm_catACA.
-  exact: perm_refl.
-by rewrite -(cat1s (f h)) -(cat1s (g h)) catA perm_cat.
-Qed.
-
-Fixpoint fsplits (A : eqType) (s : seq A) : seq (seq A * seq A)%type :=
-  if s isn't x :: xs then [:: ([::], [::])] else
-  let t := fsplits xs in
-  flatten (map (fun y => [:: (x :: y.1, y.2); (y.1, x :: y.2)]) t).
-
-Lemma fsplits_subseq (A : eqType) (s : seq A) x :
-  x \in fsplits s -> [/\ subseq x.1 s, subseq x.2 s & perm_eq (x.1 ++ x.2) s].
-elim: s x => /= [x|h t ih /= x /flattenP[/= l]].
-  by rewrite inE => /eqP ->.
-move=> /mapP[/= [x1 x2]] /ih[/= x1t x2t x1x2t ->{l}].
-rewrite !inE => /orP[|] /eqP -> /=.
-- rewrite eqxx; split => //.
-    destruct x2 as [|x21 x22] => //.
-    case: ifPn => // /eqP ?; subst x21.
-    exact: cons_subseq x2t.
-  by rewrite perm_cons.
-split.
-- destruct x1 as [|x11 x12] => //.
-  case: ifPn => // /eqP ?; subst x11.
-  exact: cons_subseq x1t.
-- by rewrite eqxx.
-- rewrite -cat_rcons -cats1.
-  by rewrite perm_catAC perm_catC perm_cons.
-Qed.
-
-Lemma fsplits_gt0 (A : eqType) (s : seq A) : (0 < size (fsplits s))%nat.
-Proof. by elim: s => // h t ih /=; destruct (fsplits t). Qed.
-
-(* NB: not used *)
-Lemma splits_fsplits (s : seq E) : splits s = arbitrary ([::], [::]) (fsplits s) :> M _.
-Proof.
-elim: s => [|h t ih]; first by rewrite /= arbitrary1.
-destruct t as [|t1 t2]; first by rewrite /= bindretf /= /arbitrary /= altC.
-rewrite [t1 :: t2]lock /= -lock ih alt_bindDr.
-have /(perm_eq_arbitrary ([::], [::])) -> : perm_eq
-  (flatten [seq [:: (h :: y.1, y.2); (y.1, h :: y.2)] | y <- fsplits (t1 :: t2)])
-  ((flatten [seq [:: (h :: y.1, y.2)] | y <- fsplits (t1 :: t2)]) ++
-   (flatten [seq [:: (y.1, h :: y.2)] | y <- fsplits (t1 :: t2)])).
-  by rewrite perm_eq_flatten_map.
-rewrite arbitrary_cat; last 2 first.
-  by apply: gt0_flatten; exact: fsplits_gt0.
-  by apply: gt0_flatten; exact: fsplits_gt0.
-by congr (_ [~] _); rewrite arbitrary_flatten //; exact: fsplits_gt0.
-Qed.
-
-(* NB: not used *)
-Lemma bind_ext_splits A (s : seq E) (f : seq E -> seq E -> M A) (m : seq E -> M A) :
-  (forall ys zs, subseq ys s -> subseq zs s -> perm_eq (ys ++ zs) s -> f ys zs = m s) ->
-  (do x <- splits s; (let '(ys, zs) := x in f ys zs))%Do = m s.
-Proof.
-move=> h.
-transitivity ((do x <- splits s; (let '(ys, zs) := x in m s))%Do).
-  rewrite splits_guard_subseq !bindA.
-  bind_ext => -[a b] /=.
-  rewrite !bindA.
-  apply: bind_ext_guard => /and3P[sa sb abs].
-  rewrite !bindretf.
-  by rewrite h.
-clear h f.
-transitivity (splits s >> m s).
-  by bind_ext => -[].
-(* TODO splits inde *)
-elim: s m => /= [m|].
-  by rewrite bindretf.
-move=> h t ih m.
-rewrite bindA.
-under eq_bind do rewrite alt_bindDl.
-rewrite alt_bindDr.
+elim: xs p a b => [/=|h t ih] p a b.
+  rewrite kleisliE apply_triple_sndE bindA.
+  under eq_bind do rewrite bindretf /=.
+  rewrite -[X in _ `<=` X]bindmret.
+  apply: refin_bindl => -[x y].
+  exact: refin_refl.
+rewrite [in X in _ `<=` X]/= -if_arg -fun_if if_pair(*if inside args*).
+apply/(refin_trans _ (ih _ _ _))/eq_refin/esym.
+rewrite -if_pair -[in LHS](if_same (h <= p) t) -if_pair(*if outside args*).
+rewrite [in LHS]kleisliE -[X in apply_triple_snd X _]qperm_idempotent fun_if.
+rewrite 2!apply_triple_snd_kleisli qperm_rcons bindA -bind_if bindA.
+rewrite [RHS]kleisliE [in RHS]apply_triple_sndE [in RHS]bindA.
+rewrite [in RHS]/apply_pair_snd /= [in RHS]bindA.
+do 2 under [RHS]eq_bind do rewrite bindretf.
+bind_ext => b'.
+rewrite -apply_triple_snd_kleisli qperm_idempotent if_bind.
+rewrite !bindA /=.
 under eq_bind do rewrite bindretf.
-under [in X in _[~]X]eq_bind do rewrite bindretf.
-by rewrite (ih (fun s => m (h :: s))) altmm.
+by under [in X in if _ then _ else X]eq_bind do rewrite bindretf.
 Qed.
 
-End fsplits.
-
-Section more_about_qperm.
-Variable M : plusMonad.
-
-(* NB: postulate return⊑perm in in Nondet.agda *)
-Lemma refin_qperm_ret (A : eqType) (s : seq A) : (Ret s : M _) `<=` qperm s.
-Proof. by rewrite -iperm_qperm; exact: refin_ret_iperm. Qed.
-
-Lemma qperm_refin_rcons (A : eqType) h (t : seq A) :
-  (Ret (rcons t h) : M _) `<=` qperm (h :: t).
-Proof. by rewrite qperm_cons_rcons; exact: refin_qperm_ret. Qed.
-
-Lemma qperm_refin_cons (A : eqType) h (t : seq A) :
-  (Ret (h :: t) : M _) `<=` qperm (rcons t h).
-Proof. by rewrite -qperm_cons_rcons; exact: refin_qperm_ret. Qed.
-
-End more_about_qperm.
-
-(* TODO: move to array_lib? *)
-Section refin_qperm_writeList.
-Variable (d : unit) (E : orderType d) (M : plusArrayMonad E Z_eqType).
-
-(* eqn 11 in mu2020flops, introduce-swap in IPartl.agda *)
-Lemma refin_qperm_writeList_cons (i : Z) x (s : seq E) :
-  writeList i (rcons s x) >> aswap (M := M) i (i + (size s)%:Z)
-  `<=`
-  qperm s >>= (fun s' => writeList (M := M) i (x :: s')).
+(* footnote 8, page 10, partl'-spec *)
+Lemma refin_qperm_partl a b p xs :
+  qperm_partl (M := M) p a b xs `<=` apply_pair_snd qperm (partl p (a, b) xs).
 Proof.
-case: s => [|h t] /=.
-  rewrite qperm_nil bindmskip bindretf addZ0 aswapxx bindmskip.
-  exact: refin_refl.
-rewrite bindA writeList_rcons -aput_writeList_rcons.
-apply: (refin_trans _ (refin_bindr _ (qperm_refin_rcons _ _ _))).
-by rewrite bindretf; exact: refin_refl.
-Qed.
-
-(* eqn 13 in mu2020flops, postulate introduce-swap in IQSort.agda *)
-Lemma refin_qperm_writeList_rcons (i : Z) x (s : seq E) :
-  writeList i (x :: s) >> aswap (M := M) i (i + (size s)%:Z)
-  `<=`
-  qperm s >>= (fun s' => writeList i (rcons s' x)).
-Proof.
-elim/last_ind: s => [|t h ih] /=.
-  rewrite qperm_nil bindmskip bindretf addZ0 aswapxx /= bindmskip.
-  exact: refin_refl.
+apply: refin_trans; last exact: refin_qperm_partl_helper.
+rewrite kleisliE.
+rewrite apply_triple_sndE.
 rewrite bindA.
-apply: (refin_trans _ (refin_bindr _ (qperm_refin_cons _ _ _))).
-by rewrite bindretf -bindA -writeList_aswap; exact: refin_refl.
+under [in X in _ `<=` X]eq_bind do rewrite bindretf.
+rewrite apply_pair_snd_uncurry3.
+rewrite -[X in X `<=` _](bindretf b ((qperm_partl p a)^~ xs)).
+exact/refin_bindr/refin_qperm_ret.
 Qed.
 
-End refin_qperm_writeList.
+End refin_qperm_partl.
+
+(* specification of ipartl *)
+Section refin_ipartl.
+Variable (d : unit) (E : orderType d) (M : plusArrayMonad E Z_eqType).
+Implicit Types i : Z.
+
+(* page 12, used in the proof of lemma 10 *)
+Let writeList_ipartl (p x : E) i (s xs : seq E) (k1 k2 : M (nat * nat)%type) :
+  writeList (i + (size s)%:Z + 1) xs >>
+    (if x <= p then writeList i (rcons s x) >> k1
+              else writeList i (rcons s x) >> k2) =
+  writeList i (s ++ x :: xs) >> aget (i + (size s)%:Z)%Z >>=
+    (fun x => if x <= p then k1 else k2) :> M _.
+Proof.
+transitivity (writeList i (s ++ x :: xs) >> if x <= p then k1 else k2 : M _).
+  case: ifPn => xp.
+  - rewrite -cat1s catA writeList_cat.
+    rewrite [in RHS]writeListC; last exact: leZZ.
+    by rewrite cats1 size_rcons natZS Z.add_1_r bindA Zplus_succ_r_reverse.
+  - rewrite -[in RHS]cat1s catA writeList_cat.
+    rewrite writeListC; last exact: leZZ.
+    by rewrite cats1 size_rcons natZS Z.add_1_r bindA Zplus_succ_r_reverse.
+rewrite bindA writeList_cat 2!bindA.
+bind_ext => -[].
+transitivity (writeList (i + (size s)%:Z)%Z (x :: xs) >> Ret x >>
+    (if x <= p then k1 else k2) : M _).
+  by rewrite bindA bindretf.
+rewrite (writeList_ret_aget _ x xs (fun x0 => if x0 <= p then k1 else k2)).
+by rewrite bindA.
+Qed.
+
+(* specification of ipartl, eqn 10 p.10 of mu2020flops *)
+Lemma refin_ipartl p i (xs zs ys : seq E) :
+  write3L i (ys, zs, xs) >>= uncurry3 (ipartl p i)
+  `<=`
+  qperm_partl (M := M) p ys zs xs >>= write2L i.
+Proof.
+elim: xs i p zs ys => [|h t ih] i p zs ys.
+  apply: eq_refin.
+  by rewrite /= bindretf cats0 bindA bindretf.
+have : (forall ys zs,
+    writeList i (ys ++ zs ++ t) >> ipartl (M := M) p i (size ys) (size zs) (size t)
+    `<=` qperm_partl p ys zs t >>= write2L i).
+  move=> {}ys {}zs; apply: (refin_trans _ (ih i p _ _)).
+  by rewrite /write3L bindA bindretf /uncurry3; exact: refin_refl.
+move=> /(@refin_qperm_partl_writeList _ E M p h ys zs t i).
+apply: refin_trans.
+apply: (@refin_trans _ _ (writeList (i + (size ys)%:Z + (size zs)%:Z + 1) t >>
+  (if h <= p
+   then writeList i (rcons (ys ++ zs) h) >>
+        aswap (i + (size ys)%:Z) (i + (size (ys ++ zs))%:Z) >>
+        ipartl p i (size ys).+1 (size zs) (size t)
+   else writeList i (rcons (ys ++ zs) h) >>
+        ipartl p i (size ys) (size zs).+1 (size t)))); last first.
+  apply: refin_bindl => -[].
+  case: ifPn => hp; last first.
+    apply: (@refin_trans _ _ (Ret (rcons zs h) >>= fun zs' =>
+        writeList i (ys ++ zs') >> ipartl p i (size ys) (size zs') (size t))); last first.
+      exact/refin_bindr/refin_qperm_ret.
+    by rewrite bindretf size_rcons rcons_cat; exact: refin_refl.
+  rewrite -[X in _ `<=` X](qperm_preserves_size2 zs (fun a b =>
+    writeList i (ys ++ h :: a) >> ipartl p i (size ys).+1 b (size t))).
+  rewrite -[in X in _ `<=` X]bindA.
+  exact/refin_bindr/refin_writeList_rcons_cat_aswap.
+rewrite -2!addZA !(addZA (size ys)%:Z) -intRD addZA -size_cat.
+rewrite bindA writeList_ipartl.
+rewrite /write3L bindA.
+under eq_bind do rewrite bindretf.
+rewrite /uncurry3 /= -addZA -intRD -size_cat.
+by rewrite bindA -catA; exact: refin_refl.
+Qed.
+
+End refin_ipartl.
 
 Section iqsort.
 Variable (d : unit) (E : orderType d) (M : plusArrayMonad E Z_eqType).
+Implicit Types i : Z.
 
+Local Obligation Tactic := idtac.
+
+(* failed attempts *)
 (*Fixpoint iqsort (i : Z) (n : nat) : M unit :=
   match n with
   | 0 => Ret tt
@@ -697,11 +650,7 @@ Variable (d : unit) (E : orderType d) (M : plusArrayMonad E Z_eqType).
             ipartl p (i + 1) 0 0 (n-1) >>= (fun '(ny, nz) => aswap i (i + ny%:Z) >> iqsort i ny))
   end.*)
 
-Local Obligation Tactic := idtac.
-
-(*
-(* fail attempt *)
-Program Fixpoint iqsort' (ni : (Z * nat))
+(*Program Fixpoint iqsort' (ni : (Z * nat))
     (f : forall (n'j : (Z * nat)), (n'j.2 < ni.2)%coq_nat -> M unit) : M unit :=
   match ni.2 with
   | 0 => Ret tt
@@ -711,8 +660,7 @@ Program Fixpoint iqsort' (ni : (Z * nat))
               f (ni.1, ny) _ >> f ((ni.1 + ny%:Z + 1)%Z, nz) _))
   end.
 Next Obligation.
-move => [i [//|n']] /= _ n [<-] p [a b] /= a' _ [-> _] _.
-*)
+move => [i [//|n']] /= _ n [<-] p [a b] /= a' _ [-> _] _.*)
 
 Program Fixpoint iqsort' ni
     (f : forall mj, (mj.2 < ni.2)%coq_nat -> M unit) : M unit :=
@@ -752,10 +700,10 @@ Proof.
   by move=> ?; congr iqsort'; apply fun_ext_dep => ?; rewrite boolp.funeqE.
 Qed.
 
-Lemma iqsort_nil (i : Z) : iqsort (i, 0) = Ret tt.
+Lemma iqsort_nil i : iqsort (i, 0) = Ret tt.
 Proof. by rewrite /iqsort Fix_eq //; exact: iqsort'_Fix. Qed.
 
-Lemma iqsort_cons (i : Z) (n : nat) : iqsort (i, n.+1) = aget i >>= (fun p =>
+Lemma iqsort_cons i (n : nat) : iqsort (i, n.+1) = aget i >>= (fun p =>
   dipartl p (i + 1)%Z 0 0 n >>= (fun nynz =>
     let ny := dipartlT1 nynz in
     let nz := dipartlT2 nynz in
@@ -763,187 +711,23 @@ Lemma iqsort_cons (i : Z) (n : nat) : iqsort (i, n.+1) = aget i >>= (fun p =>
     iqsort (i, ny) >> iqsort ((i + ny%:Z + 1)%Z, nz))).
 Proof. by rewrite [in LHS]/iqsort Fix_eq //=; exact: iqsort'_Fix. Qed.
 
-(* bottom of the page 11, used in the proof of lemma 10 *)
-Lemma refin_ipartl_tr_partl_helper (i : Z) x (ys zs : seq E) :
-  writeList i (rcons (ys ++ zs) x) >>
-    aswap (M := M) (i + (size ys)%:Z) (i + (size ys)%:Z + (size zs)%:Z)
-  `<=`
-  qperm zs >>= (fun zs' => writeList i (ys ++ x :: zs')).
-Proof.
-under [in X in _ `<=` X]eq_bind do rewrite writeList_cat.
-have -> : commute (qperm zs) _ _.
-  by move=> *; exact/commute_plus/nondetPlus_sub_qperm.
-rewrite rcons_cat writeList_cat bindA.
-apply: refin_bindl => -[].
-exact: refin_qperm_writeList_cons.
-Qed.
-
-(* page 12, used in the proof of lemma 10 *)
-Lemma writeList_ipartl (p x : E) (i : Z) (ys zs xs : seq E) :
-  writeList (i + (size ys + size zs)%:Z + 1) xs >>
-  (if x <= p
-    then writeList i (rcons (ys ++ zs) x) >>
-      aswap (i + (size ys)%:Z) (i + (size ys + size zs)%:Z) >>
-      ipartl p i (size ys + 1) (size zs) (size xs)
-    else writeList i (rcons (ys ++ zs) x) >>
-      ipartl p i (size ys) (size zs + 1) (size xs)) =
-  writeList i (ys ++ zs ++ (x :: xs)) >>
-    aget (i + (size ys + size zs)%:Z)%Z >>= (fun x =>
-    (if x <= p
-      then aswap (i + (size ys)%:Z) (i + (size ys + size zs)%:Z) >>
-        ipartl p i (size ys + 1) (size zs) (size xs)
-      else ipartl p i (size ys) (size zs + 1) (size xs))) :> M _.
-Proof.
-transitivity (writeList i (ys ++ zs ++ (x :: xs)) >>
-   if x <= p then
-     aswap (i + (size ys)%:Z) (i + (size ys + size zs)%:Z) >>
-     ipartl p i (size ys + 1) (size zs) (size xs)
-    else ipartl p i (size ys) (size zs + 1) (size xs) : M _).
-  case: ifPn => xp.
-  - rewrite catA -cat1s catA writeList_cat.
-    rewrite [in RHS]writeListC; last exact: leZZ.
-    rewrite {1}size_cat /= {1}[in RHS]intRD size_cat addZA [in RHS]bindA.
-    bind_ext => -[].
-    by rewrite cats1 bindA; bind_ext.
-  - rewrite -[in RHS]cat1s 2!catA writeList_cat.
-    rewrite writeListC; last exact: leZZ.
-    by rewrite {1}size_cat [in RHS]intRD size_cat addZA bindA cats1.
-rewrite bindA catA writeList_cat 2!bindA.
-rewrite size_cat intRD addZA.
-bind_ext => -[].
-transitivity (
-  writeList (i + (size ys)%:Z + (size zs)%:Z)%Z (x :: xs) >> Ret x >>
-  (if x <= p then
-    aswap (i + (size ys)%:Z) (i + (size ys)%:Z + (size zs)%:Z) >>
-    ipartl p i (size ys + 1) (size zs) (size xs)
-   else ipartl p i (size ys) (size zs + 1) (size xs)) : M _
-).
-  by rewrite bindA bindretf.
-rewrite (writeList_ret_aget _ x xs (fun x0 => (
-   if x0 <= p
-     then aswap (i + (size ys)%:Z) (i + (size ys)%:Z + (size zs)%:Z) >>
-       ipartl p i (size ys + 1) (size zs) (size xs)
-     else ipartl p i (size ys) (size zs + 1) (size xs)))).
-by rewrite bindA.
-Qed.
-
-(* specification of ipartl, eqn 10 p.10 of mu2020flops *)
-Lemma refin_ipartl_tr_partl p (i : Z) (xs zs ys : seq E) :
-  write3L i (ys, zs, xs) >>= uncurry3 (ipartl p i)
-  `<=`
-  tr_partl (M := M) p ys zs xs >>= write2L i.
-Proof.
-elim: xs i p zs ys => [|h t ih] i p zs ys.
-  apply: eq_refin.
-  by rewrite /= bindretf cats0 bindA bindretf.
-have : (forall ys zs,
-    writeList i (ys ++ zs ++ t) >> ipartl (M := M) p i (size ys) (size zs) (size t)
-    `<=` tr_partl p ys zs t >>= write2L i).
-  move=> {}ys {}zs.
-  apply: (refin_trans _ (ih i p _ _)).
-  rewrite /write3L bindA bindretf /uncurry3.
-  exact: refin_refl.
-move=> /(@tr_partl_writeList _ E M p h ys zs t i).
-apply: refin_trans.
-apply: (@refin_trans _ _ (writeList (i + (size ys)%:Z + (size zs)%:Z + 1) t >>
-  (if h <= p
-   then writeList i (rcons (ys ++ zs) h) >>
-        aswap (i + (size ys)%:Z) (i + (size ys)%:Z + (size zs)%:Z) >>
-        ipartl p i (size ys + 1) (size zs) (size t)
-   else writeList i (rcons (ys ++ zs) h) >>
-        ipartl p i (size ys) (size zs + 1) (size t)))); last first.
-  apply: refin_bindl => -[].
-  case: ifPn => hp; last first.
-    apply: (@refin_trans _ _ (Ret (rcons zs h) >>= fun zs' =>
-        writeList i (ys ++ zs') >> ipartl p i (size ys) (size zs') (size t))); last first.
-      apply: refin_bindr.
-      exact: refin_qperm_ret.
-    rewrite bindretf size_rcons addn1 rcons_cat.
-    exact: refin_refl.
-  rewrite -[X in _ `<=` X](qperm_preserves_size2 zs (fun a b =>
-    writeList i (ys ++ h :: a) >>
-    ipartl p i (size ys + 1) b (size t))).
-  rewrite -[in X in _ `<=` X]bindA.
-  apply: refin_bindr.
-  exact: refin_ipartl_tr_partl_helper.
-rewrite -2!addZA !(addZA (size ys)%:Z) -intRD addZA.
-rewrite -[in X in _ >> X]addZA -intRD writeList_ipartl.
-rewrite /write3L.
-rewrite bindA.
-under eq_bind do rewrite bindretf.
-rewrite /uncurry3 /=.
-rewrite bindA -addZA -intRD.
-rewrite (addn1 (size ys)) (addn1 (size zs)).
-exact: refin_refl.
-Qed.
-
-(* Lemma ipartlspec (i : Z) (p : E) ys zs xs :
-  (*write3L i >=> ipartl p i `<=` partl' p >=> write2L i.*)
-  (do x <- write3L i (ys, zs, xs); uncurry3 (ipartl p i) x)%Do `<=`
-  uncurry3 (partl' p) (ys, zs, xs) >>= (fun '(ys, zs) => write2L i (ys, zs)).
-Proof. Abort. *)
-
-(* not used 2021-09-24: first equation on page 10 *)
-(* Lemma ipartl_spec (i : Z) (p : E) (ys zs xs : seq E)
-    (ipartl : E -> Z -> (nat * nat * nat)%type -> M (nat * nat)%type) :
-  writeList i (ys ++ zs ++ xs) >> ipartl p i (size ys, size zs, size xs)
-  `<=` second qperm (partl p (ys, zs) xs) >>= write2L i.
-Proof. Abort. *)
-
-Lemma refin_qperm_tr_partl_qperm_partl a b p xs :
-  (apply_triple_snd qperm >=> uncurry3 (tr_partl p)) (a, b, xs) `<=`
-  apply_pair_snd (M := M) qperm (partl (p : E) (a, b) xs).
-Proof.
-elim: xs p a b => [/=|h t ih] p a b.
-  rewrite kleisliE apply_triple_sndE bindA.
-  under eq_bind do rewrite bindretf /=.
-  rewrite -[X in _ `<=` X]bindmret.
-  apply: refin_bindl => -[x y].
-  exact: refin_refl.
-rewrite [in X in _ `<=` X]/= -if_arg -fun_if if_pair(*if inside args*).
-apply/(refin_trans _ (ih _ _ _))/eq_refin/esym.
-rewrite -if_pair -[in LHS](if_same (h <= p) t) -if_pair(*if outside args*).
-rewrite [in LHS]kleisliE -[X in apply_triple_snd X _]qperm_idempotent fun_if.
-rewrite 2!apply_triple_snd_kleisli qperm_rcons bindA -bind_if bindA.
-rewrite [RHS]kleisliE [in RHS]apply_triple_sndE [in RHS]bindA.
-rewrite [in RHS]/apply_pair_snd /= [in RHS]bindA.
-do 2 under [RHS]eq_bind do rewrite bindretf.
-bind_ext => b'.
-rewrite -apply_triple_snd_kleisli qperm_idempotent if_bind.
-rewrite !bindA /=.
-under eq_bind do rewrite bindretf.
-by under [in X in if _ then _ else X]eq_bind do rewrite bindretf.
-Qed.
-
-(* partl'-spec *)
-Lemma refin_partl_tr_qperm_partl a b p xs :
-  tr_partl (M := M) p a b xs `<=` apply_pair_snd qperm (partl p (a, b) xs).
-Proof.
-apply: refin_trans; last exact: refin_qperm_tr_partl_qperm_partl.
-rewrite kleisliE.
-rewrite apply_triple_sndE.
-rewrite bindA.
-under [in X in _ `<=` X]eq_bind do rewrite bindretf.
-rewrite apply_pair_snd_uncurry3.
-rewrite -[X in X `<=` _](bindretf b ((tr_partl p a)^~ xs)).
-exact/refin_bindr/refin_qperm_ret.
-Qed.
-
-(* eqn 12 *)
-Lemma iqsort_slowsort (i : Z) (xs : seq E) :
+(* eqn 12 page 13 *)
+Lemma iqsort_slowsort i (xs : seq E) :
   writeList i xs >> iqsort (i, size xs) `<=` slowsort xs >>= writeList i.
 Proof.
 have [n nxs] := ubnP (size xs); elim: n xs i => // n ih xs i in nxs *.
 move: xs => [|p xs] in nxs *.
   by rewrite /= iqsort_nil slowsort_nil 2!bindretf /=; exact: refin_refl.
-(* step 1: l.342 in IQSOrt.agda, corresponds to second equation on page 13 of mu2020flops *)
-apply: (@refin_trans _ _ (tr_partl p [::] [::] xs >>= (fun '(ys, zs) =>
+(* step 1: l.342 in IQSOrt.agda,
+   corresponds to second equation on page 13 of mu2020flops *)
+apply: (@refin_trans _ _ (qperm_partl p [::] [::] xs >>= (fun '(ys, zs) =>
      writeList (i + (size ys)%:Z + 1)%Z zs >>
      qperm ys >>= (fun ys' => writeList i (rcons ys' p) >>
        iqsort (i, size ys) >>
        iqsort ((i + (size ys)%:Z + 1)%Z, size zs))))); last first.
-  (* step 1a: refin slowsort *)
-  apply: refin_trans; last by apply: refin_bindr; exact: refin_partition_slowsort.
+  (* step 1a: refin_partition_slowsort *)
+  apply: refin_trans; last first.
+    by apply: refin_bindr; exact: refin_partition_slowsort.
   rewrite bindretf.
   move pxs : (partition p xs) => tmp; case: tmp => [ys zs] in pxs *.
   (* step 1b: introduce qperm's and commute *)
@@ -951,19 +735,16 @@ apply: (@refin_trans _ _ (tr_partl p [::] [::] xs >>= (fun '(ys, zs) =>
   rewrite [X in _ `<=` X](_ : _ =
     (do zs' <- qperm zs; do ys' <- qperm ys; do ys'' <- slowsort ys';
      do zs'' <- slowsort zs'; writeList i (ys'' ++ p :: zs''))%Do); last first.
-    have -> : @commute M _ _ (qperm zs) (qperm ys) _ _.
+    have -> : commute (M := M) (qperm zs) (qperm ys) _.
       by move=> *; exact/commute_plus/nondetPlus_sub_qperm.
     bind_ext => ys'.
     rewrite !bindA; under eq_bind do rewrite !bindA.
-    have <- : @commute M _ _ (qperm zs) (slowsort ys') _ _.
+    have <- : commute (M := M) (qperm zs) (slowsort ys') _.
       by move=> *; exact/commute_plus/nondetPlus_sub_qperm.
-    bind_ext => zs'.
-    under eq_bind do rewrite bindA.
-    bind_ext => ys''.
-    by under eq_bind do rewrite bindretf.
-  (* step 1c: refine tr_partl to partl *)
-  apply: refin_trans.
-    exact/refin_bindr/refin_partl_tr_qperm_partl.
+    bind_ext => zs'; bind_ext => ys''.
+    by rewrite bindA; under eq_bind do rewrite bindretf.
+  (* step 1c: refine partl to qperm_partl *)
+  apply: refin_trans; first exact/refin_bindr/refin_qperm_partl.
   (* step 1d: execute the first qperm and record size information *)
   rewrite -partition_partl pxs bindA /=.
   under eq_bind do rewrite bindretf.
@@ -974,10 +755,11 @@ apply: (@refin_trans _ _ (tr_partl p [::] [::] xs >>= (fun '(ys, zs) =>
   rewrite ![in X in X `<=` _]bindA.
   have <- : commute (qperm ys) (writeList (i + (size ys)%:Z + 1) zs' : M _) _.
     by move=> T f; exact/commute_plus/nondetPlus_sub_qperm.
-  (* step 1f: qperm_preserves_size2, execute the second qperm and record size information *)
+  (* step 1f: qperm_preserves_size2,
+     execute the second qperm and record size information *)
   rewrite (qperm_preserves_size2 ys (fun a b =>
-    (writeList (i + b%:Z + 1) zs' >> (writeList i (rcons a p) >> iqsort (i, b) >>
-    iqsort ((i + b%:Z + 1)%Z, size zs'))))).
+    (writeList (i + b%:Z + 1) zs' >> (writeList i (rcons a p) >>
+      iqsort (i, b) >> iqsort ((i + b%:Z + 1)%Z, size zs'))))).
   rewrite bind_qperm_guard [in X in _ `<=` X]bind_qperm_guard (*NB: interesting?*).
   apply: refin_bindl => ys'.
   apply: refin_bind_guard => /eqP ysys'.
@@ -1002,7 +784,8 @@ apply: (@refin_trans _ _ (tr_partl p [::] [::] xs >>= (fun '(ys, zs) =>
     exact/commute_plus/nondetPlus_sub_slowsort.
   rewrite (slowsort_preserves_size2 _
     (fun a b => writeList (i + b%:Z + 1) zs' >>
-      (writeList (i + b%:Z) [:: p] >> writeList i a >> iqsort ((i + b%:Z + 1)%Z, size zs')))).
+      (writeList (i + b%:Z) [:: p] >> writeList i a >>
+        iqsort ((i + b%:Z + 1)%Z, size zs')))).
   rewrite bind_slowsort_guard [in X in _ `<=` X]bind_slowsort_guard.
   apply: refin_bindl => ys''.
   apply: refin_bind_guard => /eqP ys'ys''.
@@ -1019,7 +802,7 @@ apply: (@refin_trans _ _ (tr_partl p [::] [::] xs >>= (fun '(ys, zs) =>
   move: nxs; rewrite /= ltnS; apply: leq_ltn_trans.
   by rewrite -zszs' -(size_partition p xs) pxs /= leq_addl.
 (* step 2: introduce_aswap_rcons *)
-apply: (@refin_trans _ _ (tr_partl p [::] [::] xs >>= (fun '(ys, zs) =>
+apply: (@refin_trans _ _ (qperm_partl p [::] [::] xs >>= (fun '(ys, zs) =>
      writeList (i + (size ys)%:Z + 1) zs >>
      (writeList i (p :: ys) >> aswap i (i + (size ys)%:Z)) >>
      (iqsort (i, size ys)) >> iqsort ((i + (size ys)%:Z + 1)%Z, size zs)))); last first.
@@ -1031,9 +814,9 @@ apply: (@refin_trans _ _ (tr_partl p [::] [::] xs >>= (fun '(ys, zs) =>
   rewrite -2![in X in X `<=` _]bindA.
   rewrite (bindA _ (fun _ => iqsort _) (fun _ => iqsort _)).
   apply: refin_bindr.
-  exact: refin_qperm_writeList_rcons.
+  exact: refin_writeList_cons_aswap.
 (* step 3: commute *)
-rewrite [X in _ `<=` X](_ : _ = tr_partl p [::] [::] xs >>= (fun '(ys, zs) =>
+rewrite [X in _ `<=` X](_ : _ = qperm_partl p [::] [::] xs >>= (fun '(ys, zs) =>
      aput i p >> writeList (i + 1)%Z (ys ++ zs) >>
      (aswap i (i + (size ys)%:Z)) >>
      (iqsort (i, size ys)) >> iqsort ((i + (size ys)%:Z + 1)%Z, size zs))); last first.
@@ -1043,16 +826,16 @@ rewrite [X in _ `<=` X](_ : _ = tr_partl p [::] [::] xs >>= (fun '(ys, zs) =>
   by rewrite /= bindA writeList_cat addZAC !bindA.
 (* step 4: commute *)
 rewrite [X in _ `<=` X](_ : _ = aput i p >>
-   tr_partl p [::] [::] xs >>= (fun '(ys, zs) =>
+   qperm_partl p [::] [::] xs >>= (fun '(ys, zs) =>
    ( writeList (i + 1)%Z (ys ++ zs) >>
      (aswap i (i + (size ys)%:Z)) >>
      (iqsort (i, size ys)) >> iqsort ((i + (size ys)%:Z + 1)%Z, size zs)))); last first.
-  rewrite [RHS]bindA -(_ : commute (tr_partl p [::] [::] xs) (aput i p) _); last first.
-    exact/commute_plus/nondetPlus_sub_tr_partl.
+  rewrite [RHS]bindA -(_ : commute (qperm_partl p [::] [::] xs) (aput i p) _); last first.
+    exact/commute_plus/nondetPlus_sub_qperm_partl.
   by bind_ext=> -[a b]; rewrite !bindA.
 (* step 5 *)
 rewrite [X in _ `<=` X](_ : _ = aput i p >>
-  tr_partl p [::] [::] xs >>= (fun '(ys, zs) =>
+  qperm_partl p [::] [::] xs >>= (fun '(ys, zs) =>
     write2L (i + 1)%Z (ys, zs)) >>= (fun '(sys, szs) =>
      (aswap i (i + sys%:Z)) >>
      (iqsort (i, sys)) >> iqsort ((i + (sys)%:Z + 1)%Z, szs))); last first.
@@ -1060,13 +843,12 @@ rewrite [X in _ `<=` X](_ : _ = aput i p >>
   rewrite 2!bindA /write2L [RHS]bindA; bind_ext => -[].
   by rewrite bindretf bindA.
 rewrite {nxs}.
-(* step 6: refin_ipartl_tr_partl *)
+(* step 6: refin_ipartl_qperm_partl *)
 rewrite [in X in _ `<=` X](bindA (aput i p)).
 apply: refin_trans; last first.
   rewrite bindA.
   apply: refin_bindl => ttt.
-  apply: refin_bindr.
-  exact: refin_ipartl_tr_partl.
+  exact/refin_bindr/refin_ipartl.
 (* step 7 *)
 rewrite -[in X in _ `<=` X]bindA.
 rewrite (_ : aput i p >> _ = (writeList i (p :: xs) >> Ret p) >>=
